examples/ssr/SystemF_CBV.v
@@ -1,63 +1,621 @@
 (** * Normalization of Call-By-Value System F *)
 
-Require Import ssreflect ssrfun ssrbool eqtype ssrnat seq.
-Require Import AutosubstSsr Context.
+Require Import Autosubst.Autosubst_Basics Autosubst.Autosubst_Derive Autosubst.Autosubst_MMap.
 
+(* Set Universe Polymorphism. *)
 Set Implicit Arguments.
 Unset Strict Implicit.
 Unset Printing Implicit Defensive.
 
 (** **** Definitions *)
 
-Inductive type : Type :=
-| TyVar (x : var)
-| Arr   (A B : type)
-| All   (A : {bind type}).
+Require Import Decidable.
 
-Inductive term :=
-| TeVar (x : var)
-| Abs   (A : type) (s : {bind term})
-| App   (s t : term)
-| TAbs  (s : {bind type in term})
-| TApp  (s : term) (A : type).
+Definition _bind {sort : Set} (o : sort) (T : Type) (n : nat) := T.
+Arguments _bind / {sort} o T n.
 
-(** **** Substitution Lemmas *)
 
-Instance Ids_type : Ids type. derive. Defined.
-Instance Rename_type : Rename type. derive. Defined.
-Instance Subst_type : Subst type. derive. Defined.
+Notation "{ 'bind' n 'of' T1 'in' T2 }" :=
+  (_bind T1 T2 n) (at level 0,
+   format "{ 'bind'  n  'of'  T1  'in'  T2 }") : bind_scope.
 
-Instance SubstLemmas_type : SubstLemmas type. derive. Qed.
+Notation "{ 'bind' T1 'in' T2 }" :=
+  (_bind T1 T2 1) (at level 0,
+   format "{ 'bind'  T1  'in'  T2 }") : bind_scope.
 
-Instance HSubst_term : HSubst type term. derive. Defined.
+Open Scope bind_scope.
 
-Instance Ids_term : Ids term. derive. Defined.
-Instance Rename_term : Rename term. derive. Defined.
-Instance Subst_term : Subst term. derive. Defined.
 
-Instance HSubstLemmas_term : HSubstLemmas type term. derive. Qed.
-Instance SubstHSubstComp_type_term : SubstHSubstComp type term. derive. Qed.
 
-Instance SubstLemmas_term : SubstLemmas term. derive. Qed.
+(* Goal forall s t,  Arr s t = Var Ty 3 -> s = t. intros. inversion H. *)
+
+Class Vector (sort : Type) :=
+  {
+    vec : (sort -> Type) -> Type;
+    getV {T : sort -> Type} : vec T -> forall o : sort, T o;
+    newV {T : sort -> Type} : (forall o : sort, T o) -> vec T;
+    getV_newV {T : sort -> Type} (f : forall o, T o) : getV (newV f) = f 
+  }.
+
+Notation substitution term := (vec (fun o => var -> term o)).
+
+Section SubstOps.
+  Context {sort : Type}
+          {dec_eq_sort : forall a b : sort, Dec (a = b)}.
+
+  Definition upd (o : sort) {T : sort -> Type} (x : T o) (f : forall o, T o) : forall o, T o.
+    refine (fun o' => match decide (o = o') with
+                       | left p => _
+                       | right _ => f o' end).
+    subst. exact x.
+  Defined.
+  Global Arguments upd !o {T} x f !o0/.
+  Context {Vector_sort : Vector sort}.
+
+  Lemma upd_upd o {T : sort -> Type} (x y n: T o) f : upd o x (upd o y f) = upd o x f.
+  Proof.  f_ext. intro o'. unfold upd. decide(o = o'); now subst.  Qed.
+
+  Definition updV (o : sort) {term : sort -> Type} (sigma : var -> term o) (v : substitution term) : substitution term :=
+    newV (upd o sigma (getV v)).
+  Global Arguments updV o {term} sigma v.
+
+  Definition mapV {term : sort -> Type} (f : forall o, (var -> term o) -> (var -> term o)) (v : substitution term) : substitution term :=
+    newV (fun o => f o (getV v o)).
+  Global Arguments mapV {term} f v.
+  
+  Definition funcompV {term : sort -> Type} (v : substitution term) (f : forall o, term o -> term o) : substitution term := @mapV term (fun o x => x >>> (f o)) v.
+  Global Arguments funcompV {term} v f.
+
+  Context {term : sort -> Type}.
+
+  Class Ids := ids : (forall o, var -> term o).
+  Global Arguments ids {Ids} o x.
+  Class Rename := rename : (sort -> var -> var) -> forall o : sort, term o -> term o.
+  Global Arguments rename {Rename} xi [o] !s/.
+  Class Subst := subst : (substitution term) -> forall {o : sort}, term o -> term o.
+  Global Arguments subst {Subst} sigma [o] !s/.
+
+End SubstOps.
+
+Arguments Ids {sort} term.
+Arguments Rename {sort} term.
+Arguments Subst {sort} {Vector_sort} term.
+(* Notation subst := (_subst (Subst:=$(exact _ )$)). *)
+
+
+Definition dfuncomp2 {A B C D} (f : forall a : A, B -> C) (g : forall a : A, C -> D a) a := f a >>> g a .
+Arguments dfuncomp2 {A B C D} f g a / x.
+
+Notation "f >>2 g" := (dfuncomp2 f g)
+  (at level 56, left associativity) : subst_scope.
+
+
+Notation "v |>> f" := (funcompV v f)
+  (at level 56, left associativity) : msubst_scope.
+
+
+Notation "sigma >> tau" := (sigma >>> subst tau)
+  (at level 56, left associativity) : subst_scope.
+
+
+(* Notation "s .[ ( sigma_1 ; sigma_2 ; .. ; sigma_n ) ]" := *)
+(*   (subst ((fun p : (fun T => prod ( .. ( prod ((fun _ => var -> T _) sigma_1) ((fun _ => var -> T _) sigma_2) ) .. ) ((fun _ => var -> T _) sigma_n)) _ => p) (pair ( .. (pair sigma_1 sigma_2) ..) sigma_n)) s) *)
+(*   (at level 2, left associativity, *)
+(*    format "s '[ ' .[ ( sigma_1 ; sigma_2 ;  .. ;  sigma_n ')' ] ']'") : msubst_scope. *)
+
+
+Notation "s .[ sigma ]" :=  (subst sigma s)
+  (at level 2, left associativity,
+   format "s '[ ' .[ sigma ] ']'") : msubst_scope.
+
+
+Delimit Scope msubst_scope with msubst.
+Open Scope msubst_scope.
+
+
+Section Classes.
+
+  Context {sort : Type}
+          {dec_eq_sort : forall a b : sort, Dec (a = b)}.
+  Context {Vector_sort : Vector sort}.
+
+  Context (term : sort -> Type).
+  
+  Context {Ids_term : Ids term} {Rename_term : Rename term} {Subst_term : Subst term}.
+  
+  Definition upren (o : sort) (xi : sort -> var -> var) : sort -> var -> var :=
+    upd o (0 .: (xi o >>> S)) xi.
+  Global Arguments upren o xi o' x/.
+
+  Definition idr : sort -> var -> var := fun _ => id.
+  
+  Definition ren (xi : sort -> var -> var) := newV (xi >>2 ids).
+
+  Definition up (o : sort) (sigma : substitution term) : substitution term :=
+    updV o (ids o 0 .: getV sigma o >>> rename (upd o (+1) idr) (o := _)) (sigma |>> rename (upd o (+1) idr)).
+  Global Arguments up o sigma : simpl never.
+
+  
+  Lemma up_comp_ren_subst o xi sigma :
+    up o (newV (xi >>2 getV sigma)) = newV (upren o xi >>2 getV (up o sigma)).
+  Proof.
+    unfold up. unfold updV. f_equal. f_ext. intros o'. f_ext. simpl.
+    unfold funcompV. unfold mapV. rewrite ?getV_newV.
+    unfold upd.
+    decide (o=o'); simpl.
+    - unfold eq_rect_r. unfold eq_rect. destruct eq_sym. now intros [|x].
+    - now intros [|x].
+Qed.  
+
+Lemma up_comp_ren_subst_n o xi sigma n :
+  iterate (up o) n (newV (xi >>2 getV sigma)) = newV (iterate (upren  o) n xi >>2 getV (iterate (up o) n sigma)) .
+Proof.
+  induction n. reflexivity. rewrite !iterate_S, IHn. apply up_comp_ren_subst.
+Qed.
+  
+ Class SubstLemmas  :=
+    {
+      rename_subst (xi : sort -> var -> var) (o : sort) (s : term o) :
+        rename xi s = subst (ren xi) s;
+      subst_id (o : sort) (s : term o) :
+        s.[newV ids] = s;
+      id_subst (sigma : substitution term) (o : sort) (x : var) :
+        (ids o x).[sigma] = getV sigma o x;
+      subst_comp (sigma tau : substitution term) (o : sort) (s : term o) :
+        s.[sigma].[tau] = s.[sigma |>> subst tau]
+    }.
+  
+End Classes.
+Arguments up {sort dec_eq_sort Vector_sort term Ids_term Rename_term} o sigma : simpl never.
+Arguments ren {sort Vector_sort term Ids_term} xi : simpl never.
+Arguments SubstLemmas {sort Vector_sort} term {Ids_term Rename_term Subst_term}.
+
+Arguments idr {sort} o/ x. 
+
+Arguments newV : simpl never.
+Arguments getV {sort Vector T} !v o.
+Arguments funcompV {sort Vector_sort term} !v f. 
+    
+Inductive sort := Ty | Ter.
+
+Instance decide_eq_sort (o1 o2 : sort) : Dec (o1 = o2). gen_Dec_eq. Defined.
+
+Instance Vector_sort : Vector sort :=
+  {
+    vec := (fun T => T Ty * T Ter)%type;
+    getV T v := let (v1, v2) := v in
+               fun o => match o with
+                         | Ty => v1
+                         | Ter => v2
+                       end;
+    newV T f := (f Ty, f Ter)
+  }.
+Proof. intros. f_ext. now destruct 0. Defined.
+
+Inductive term : sort -> Type :=
+| Var  (o : sort) (x : var) : term o
+| Arr    (A B : term Ty) : term Ty
+| All    (A : {bind Ty in (term Ty)}) : term Ty
+| Abs    (A : term Ty) (s : {bind Ter in term Ter}) : term Ter
+| App    (s t : term Ter) : term Ter
+| TAbs   (s : {bind Ty in term Ter}) : term Ter
+| TApp   (s : term Ter) (A : term Ty) : term Ter.
+
+Instance Ids_term : Ids term := Var.
+
+Ltac derive_Rename :=
+  match goal with [ |- Rename ?term ] =>
+    hnf; fix inst 3; change _ with (Rename term) in inst;
+    intros xi o s; change (annot (term o) s); destruct s;
+    match goal with
+      | [ x : var |- annot _ (?Var _ _)] => exact (Var o (xi o x))
+      | [ |- annot _ ?t ] =>
+        let rec map s :=
+            (match s with
+               | ?s1 ?s2 =>
+                 let s1 := map s1 in
+                 let T  := typeof s2 in
+                 let s2 :=
+                     match T with
+                       | term _ => constr:(rename xi s2)
+                       | var  => constr:(xi s2)
+                       | @_bind _ ?o _ 1 => constr:(rename (upren o xi) s2)
+                       | @_bind _ ?o _ ?n =>
+                           constr:(rename (iterate (upren o) n xi) s2)
+                       | _ => s2
+                     end in
+                 constr:(s1 s2)
+               | _ => s
+             end) in
+        let t := map t in exact t
+    end
+  end.
+
+Hint Extern 0 (Rename _) => derive_Rename : derive.
+
+
+Instance Rename_term : Rename term. derive_Rename. Show Proof. Defined.
+
+Ltac has_var s :=
+  match s with
+    | ?s1 ?s2 =>
+      match has_var s1 with
+        | Some ?x => constr:(Some x)
+        | _ =>
+          match typeof s2 with
+            | var => constr:(Some s2)
+            | _ => None
+          end
+      end
+    | _ => None
+  end.
+
+Ltac derive_Subst :=
+  match goal with [ |- Subst ?term ] =>
+    require_instance (Rename term);
+    hnf; fix inst 3; change _ with (Subst term) in inst;
+    intros sigma o s; change (annot (term o) s); destruct s;
+    match goal with
+      | [ x : var |- annot _ (?Var _ _)] => 
+        exact (getV sigma o x)
+      | [ |- annot _ ?t ] =>
+        let rec map s :=
+            (match s with
+               | ?s1 ?s2 =>
+                 let s1 := map s1 in
+                 let T  := typeof s2 in
+                 let s2 :=
+                   match T with
+                     | term _ => constr:(s2.[sigma])
+                     | _bind ?o _ 1 => constr:(s2.[up o sigma])
+                     | _bind ?o _ ?n => constr:(s2.[iterate (up o) n sigma])
+                   end in
+                 constr:(s1 s2)
+               | _ => s
+             end) in
+        let t := map t in exact t
+    end
+  end.
+Hint Extern 0 (Subst _) => derive_Subst : derive.
+Arguments eq_rect_r {A x} P H {y} H0/.
+
+Definition foo I := Subst (Vector_sort := I) term.
+
+Instance Subst_term : Subst term.
+derive. Show Proof. Defined.
+
+Goal forall (a : var -> term Ty) (b : var -> term Ter), (subst (a,b) (ids Ter 0)) = (ids Ter 0).[pair a b]. trivial. Qed.
+
+Lemma iter_param {A B} (f : A -> A) (g : B -> B) (h : A -> B) :
+  (forall x, g (h x) = h (f x)) ->
+  (forall x n, iterate g n (h x) = h (iterate f n x)).
+Proof.
+  intros E x n. induction n. reflexivity. now rewrite !iterate_S, IHn, E.
+Qed.
+
+Require Import FunctionalExtensionality.
+
+Ltac casedist_up := intros o; intros; simpl; destruct o; unfold up; unfold ren; unfold newV; unfold funcompV; simpl; f_equal; f_ext; (intros [|x]); reflexivity.
+
+Lemma up_comp_subst_ren_n_internal :
+  (forall o sigma xi, up o (sigma |>> rename xi) = up o sigma |>> rename (upren o xi))->
+  (forall o sigma xi n,
+    iterate (up o) n (sigma |>> rename xi) = iterate (up o) n sigma |>> rename (iterate (upren o) n xi)).
+Proof.
+  intros E o sigma xi n. induction n. reflexivity. rewrite !iterate_S, IHn.
+  apply E.
+Qed.
+
+Ltac derive_SubstLemmas :=
+  lazymatch goal with
+    [ |- 
+@SubstLemmas ?sort ?Vector_sort ?term ?Ids_term ?Rename_term ?Subst_term] =>
+
+    (* rename subst *)
+
+assert (rename_subst :
+          forall o xi (s : term o), rename xi s = subst (ren xi) s)
+  by (
+      assert (up_upren :
+                forall o xi, up o (ren xi) = ren (upren o xi))
+      by casedist_up;
+      assert (up_upren_n :
+                forall o xi n, iterate (up o) n (ren xi) = ren (iterate (upren o) n xi))
+        by (intros; now apply iter_param);
+      fix ih 3; intros o xi s; destruct s; (try destruct o); try reflexivity; try (simpl; f_equal ;
+                                                                                  try apply mmap_ext; intros; rewrite ?up_upren, ?up_upren_n; now apply ih));
+
+  (* subst id *)
+
+  assert (subst_id : forall o (s : term o), subst (newV ids) s = id s)
+  by (
+      assert (up_id : forall o, up o (newV ids) = newV ids) by casedist_up;
+      assert (up_id_n : forall o n, iterate (up o) n (newV ids) = (newV ids)) by (intros; now apply iter_fp);
+      fix ih 2; intros o s; destruct s; simpl in *; repeat match goal with [o : sort |- _ ] => destruct o end; f_equal; try reflexivity;
+      rewrite ?up_id, ?up_id_n; try apply mmap_id_ext; intros; apply ih);
+  
+  (* subst comp *)
+  
+  assert (ren_subst_comp :
+            forall (xi : sort -> var -> var) sigma o (s : term o), (rename xi s).[sigma] = s.[newV (xi >>2 getV sigma)])
+    by (
+        fix ih 4; intros xi sigma o s; destruct s; simpl; trivial; try
+        (now destruct o); now ( 
+        f_equal; rewrite ?up_comp_ren_subst, ?up_comp_ren_subst_n, ?mmap_comp;
+               try apply mmap_ext; intros; try apply ih)
+      );
+  
+  assert (subst_ren_comp : forall sigma xi o (s : term o),
+                             rename xi s.[sigma] = s.[sigma |>> rename xi])
+    by (
+        
+        assert (up_comp_subst_ren :
+                  forall o sigma xi, up o (sigma |>> rename xi) = up o sigma |>> rename (upren o xi))
+        by (
+            intros o sigma xi; destruct sigma; destruct o; simpl; unfold up; unfold funcompV; simpl; repeat first[f_ext | f_equal]; destruct 0; trivial; simpl; try now repeat rewrite rename_subst, ren_subst_comp);
+        
+        assert (up_comp_subst_ren_n :
+                  forall o sigma xi n, iterate (up o) n (sigma |>> rename xi) = iterate (up o) n sigma |>> rename (iterate (upren o) n xi))
+          by (
+              apply up_comp_subst_ren_n_internal; apply up_comp_subst_ren);
+        fix ih 4; intros sigma xi o s; destruct s; try reflexivity; simpl;
+        f_equal; rewrite ?up_comp_subst_ren, ?up_comp_subst_ren_n, ?mmap_comp;
+        first [now destruct o | intros; apply ih]                          
+      );
+  
+assert (subst_comp :
+          forall o sigma tau (s : term o), s.[sigma].[tau] = s.[sigma |>> subst tau])
+  by (
+      assert (up_comp : forall o sigma tau, up o (sigma |>> subst tau) = up o sigma |>> subst (up o tau))
+      by (
+          intros o sigma tau; destruct o; unfold up; unfold funcompV; simpl;
+          repeat first[f_ext | f_equal] ;
+          destruct 0; simpl; trivial; rewrite ?subst_ren_comp; now rewrite ?ren_subst_comp
+        );
+      
+      (* assert (up_comp_n : forall sigma tau n, upn n (sigma >> tau) = upn n sigma >> upn n tau) *)
+      (*  by (apply up_comp_n_internal; apply up_comp); *)
+      fix ih 4; intros o sigma tau s; destruct s; simpl; trivial; simpl; f_equal;
+      rewrite ?up_comp, (*?up_comp_n, *) ?mmap_comp;
+      try apply mmap_ext; intros; solve[ now destruct o | apply ih]
+    );
+constructor; hnf; intros;
+[apply rename_subst|apply subst_id|reflexivity|apply subst_comp]
+  end.
+Hint Extern 0 (SubstLemmas _) => derive_SubstLemmas : derive.
+
+
+Instance SubstLemmas_term : SubstLemmas term.
+ derive. Qed.
+  
+
 
 (** **** Call-by value reduction *)
 
-Inductive eval : term -> term -> Prop :=
-| eval_beta (A : type) (s t u1 u2 v : term) :
-    eval s (Abs A u1) -> eval t u2 -> eval u1.[u2/] v -> eval (App s t) v
-| eval_tbeta (B : type) (s A v : term) :
-    eval s (TAbs A) -> eval A.|[B/] v -> eval (TApp s B) v
-| eval_abs (A : type) (s : term) :
+
+Inductive eval : term Ter -> term Ter -> Prop :=
+| eval_beta (A : term Ty) (s t u1 u2 v : term Ter) :
+    eval s (Abs A u1) -> eval t u2 -> eval (u1.[(ids Ty, u2 .: ids Ter)]) v -> eval (App s t) v
+| eval_tbeta (B : term Ty) (s A v : term Ter) :
+    eval s (TAbs A) -> eval A.[(B .: ids Ty, ids Ter)] v -> eval (TApp s B) v
+| eval_abs (A : term Ty) (s : term Ter) :
     eval (Abs A s) (Abs A s)
-| eval_tabs (A : term) :
+| eval_tabs (A : term Ter) :
     eval (TAbs A) (TAbs A).
 Hint Resolve eval_abs eval_tabs.
 
+
+
+(** Derived substitution lemmas. *)
+
+Section LemmasForSubst.
+
+  Context {sort : Type}
+          {dec_eq_sort : forall a b : sort, Dec (a = b)}
+          {Vector_sort : Vector sort}
+          {term : sort -> Type}
+          {Ids_term : Ids term} {Rename_term : Rename term} {Subst_term : Subst term}
+          {SubstLemmas_term : SubstLemmas term}.
+
+Implicit Types (sigma tau theta :  substitution term) (xi : sort -> var -> var).
+
+Lemma rename_substX xi : rename xi = subst (ren xi).
+Proof. repeat(f_ext; intros). now apply rename_subst. Qed.
+
+(* Variable (o : sort) (sigma : vec (fun o : sort => var -> term o)) (s : term o) . *)
+
+(* Goal up o sigma = up o sigma. unfold up. simpl. rewrite rename_substX. simpl. *)
+
+Lemma upX o (sigma : substitution term) :
+  up o sigma =
+  updV o (ids o 0 .: getV sigma o >>> subst (ren (upd o (+1) idr)) (o:=o))
+     (sigma |>> subst (ren (upd o (+1) idr))).
+Proof. unfold up. now rewrite rename_substX. Qed.
+
+Lemma id_scompX sigma o : ids o >>> subst sigma (o := o) = getV sigma o.
+Proof. f_ext. now eapply id_subst. Qed.
+
+Lemma id_scompR {A} sigma o (f : term o -> A) :
+  ids o >>> (subst sigma (o := o) >>> f) = getV sigma o >>> f.
+Proof. now rewrite <- compA, id_scompX. Qed.
+
+Lemma subst_idX : subst (newV ids) = fun o (s : term o) => s.
+Proof. f_ext. intro. f_ext. now eapply subst_id. Qed.
+
+Lemma subst_compI sigma tau o (s : term o) :
+  s.[sigma].[tau] = s.[sigma |>> subst tau].
+Proof. now eapply subst_comp. Qed.
+
+Lemma subst_compX sigma tau o :
+  subst sigma (o := o) >>> subst tau (o := o) = subst (sigma |>> subst tau) (o := o).
+Proof. f_ext. intro. now eapply subst_comp. Qed.
+
+(* Lemma subst_compR {A} sigma tau (f : _ -> A) : *)
+(*   subst sigma >>> (subst tau >>> f) = subst (sigma >>> subst tau) >>> f. *)
+(* Proof. now rewrite <- subst_compX. Qed. *)
+
+Lemma fold_ren_cons (x : var) (xi : var -> var) o :
+  ids o x .: (xi >>> ids o) = (x .: xi) >>> ids o.
+Proof. now rewrite scons_comp. Qed.
+
+(* unfold upn *)
+
+(* Lemma upnSX n sigma : *)
+(*   upn (S n) sigma = ids 0 .: upn n sigma >>> subst (ren (+1)). *)
+(* Proof. *)
+(*   unfold iterate; now rewrite upX. *)
+(* Qed. *)
+
+(* Lemma upnSE n sigma : *)
+(*   upn (S n) sigma = ids 0 .: upn n sigma >> ren (+1). *)
+(* Proof. *)
+(*   now rewrite upnSX. *)
+(* Qed. *)
+
+(* Lemma upn0 sigma : upn 0 sigma = sigma. *)
+(* Proof. reflexivity. Qed. *)
+
+
+
+(* fold up *)
+
+(* Lemma fold_up k sigma : *)
+(*   ids k .: sigma >> ren (+S k) = up sigma >> ren (+k). *)
+(* Proof. *)
+(*   unfold scomp, ren. rewrite upX; fsimpl; rewrite id_subst, subst_compX; simpl; fsimpl. *)
+(*   unfold ren. fsimpl. rewrite id_scompX. now fsimpl. *)
+(* Qed. *)
+
+(* Lemma fold_up0 sigma : *)
+(*   sigma >> ren (+0) = sigma. *)
+(* Proof. *)
+(*   unfold scomp, ren. fsimpl. now rewrite subst_idX. *)
+(* Qed. *)
+
+
+
+(* combine up *)
+
+(* Lemma fold_up_up sigma : up (up sigma) = upn 2 sigma. *)
+(* Proof. reflexivity. Qed. *)
+
+(* Lemma fold_up_upn n sigma : up (upn n sigma) = upn (S n) sigma. *)
+(* Proof. reflexivity. Qed. *)
+
+(* Lemma fold_upn_up n sigma : upn n (up sigma) = upn (S n) sigma. *)
+(* Proof. now rewrite iterate_Sr. Qed. *)
+
+End LemmasForSubst.
+
+
+Ltac autosubst_typeclass_normalize :=
+  mmap_typeclass_normalize;
+  repeat match goal with
+  | [|- context[ids ?x]] =>
+    let s := constr:(ids x) in progress change (ids x) with s
+  | [|- appcontext[ren ?xi]] =>
+    let s := constr:(ren xi) in progress change (ren xi) with s
+  | [|- appcontext[rename ?xi]] =>
+    let s := constr:(rename xi) in progress change (rename xi) with s
+  | [|- appcontext[subst ?sigma]] =>
+    let s := constr:(subst sigma) in progress change (subst sigma) with s
+  end.
+
+Ltac autosubst_typeclass_normalizeH H :=
+  mmap_typeclass_normalizeH H;
+  repeat match typeof H with
+  | context[ids ?x] =>
+    let s := constr:(ids x) in progress change (ids x) with s in H
+  | appcontext[ren ?xi] =>
+    let s := constr:(ren xi) in progress change (ren xi) with s in H
+  | appcontext[rename ?xi] =>
+    let s := constr:(rename xi) in progress change (rename xi) with s in H
+  | appcontext[subst ?sigma] =>
+    let s := constr:(subst sigma) in progress change (subst sigma) with s in H
+  end.
+
+
+Ltac autosubst_unfold_up :=
+  rewrite ?upX (*, ?upnSX; *)
+  (* repeat match goal with *)
+  (* | [|- context[upn 0 ?sigma]] => change (upn 0 sigma) with sigma *)
+  (* end *).
+
+Ltac autosubst_unfold_upH H :=
+  rewrite ?upX(* , ?upnSX*) in H(*; *)
+  (* repeat match typeof H with *)
+  (* | context[upn 0 ?sigma] => change (upn 0 sigma) with sigma *)
+  (* end *).
+
+Ltac autosubst_unfold :=
+  autosubst_typeclass_normalize; autosubst_unfold_up;
+  rewrite ?(@rename_substX _ _ _ _ _ _); unfold ren, upren.
+
+Ltac autosubst_unfoldH H :=
+  autosubst_typeclass_normalizeH H; autosubst_unfold_upH H;
+  rewrite ?(@rename_substX _ _ _ _ _ _) in H; unfold ren, upren in H.
+
+Ltac etaReduce := repeat lazymatch goal with [|- context[fun x => ?f x]] => change (fun x => f x) with f end.
+
+Ltac etaReduceH H := repeat lazymatch goal with [H : context[fun x => ?f x] |- _ ] => change (fun x => f x) with f in H end.
+
+Ltac asimpl :=
+  let subst_idX_inst := fresh "E" in
+  lazymatch goal with [|- appcontext[@subst _ _ _ ?Subst_term]] =>
+pose proof (@subst_idX _ _ _ _ _ Subst_term _) as subst_idX_inst;
+  unfold newV in subst_idX_inst;
+  simpl in subst_idX_inst
+  end; 
+  simpl; autosubst_unfold; repeat first
+  [ progress (
+      simpl; unfold _bind, ren, funcompV; fsimpl; autosubst_unfold_up;
+      autorewrite with autosubst;
+      rewrite ?id_scompX, ?id_scompR, ?subst_compX,
+      (* ?subst_compR, *) ?id_subst, ?subst_id, ?subst_compI, ?subst_idX_inst
+      (* repeat match goal with [|- appcontext[@subst ?sort ?vec ?term ?Subst ?sigma]] => *)
+      (*                        replace (@subst sort vec term Subst sigma ) with (fun o : sort =>  @id (term o)) by eauto using subst_idX end *)
+    )
+  | fold_id];
+(* fold_ren; fold_comp; fold_up *)
+  clear subst_idX_inst
+.
+
+Ltac asimplH H :=
+  simpl in H; autosubst_unfoldH H; repeat first
+  [ progress (
+        simpl in H;
+        unfold _bind, ren, funcompV in H; fsimplH H;
+        autosubst_unfold_upH H;
+        autorewrite with autosubst in H;
+        rewrite ?id_scompX, ?id_scompR, ?subst_compX,
+        (* ?subst_compR, *) ?id_subst, ?subst_id in H;
+        repeat setoid_rewrite subst_compI in H;
+        let E := constr:(@subst_idX _ _ _ _ _ _) in rewrite ?(E _ _) in H (* I have no idea why this works ... well, it does no longer in Coq 8.5*)
+      )
+  | fold_idH H](* ; *)
+(* fold_ren; fold_comp; fold_up *).
+
+Lemma eta {A : Type} (f : var -> A): (fun b : var => f b) = f. reflexivity. Qed.
+
+Lemma eval_subst s t : eval s t -> forall (sigma : var -> term Ty) (tau : var -> term Ter) , eval s.[(sigma, tau)] t.[(sigma, tau)].
+Proof.
+  simpl.
+  induction 1; intros; eauto using eval.
+  - econstructor; eauto.
+    fsimpl. asimpl.
+    specialize (IHeval3 sigma tau).
+    asimplH IHeval3.
+    assumption.
+  - econstructor; eauto. asimpl.
+    specialize (IHeval2 sigma tau).
+    asimplH IHeval2.
+    assumption.
+Qed.
+
 (** **** Syntactic typing *)
 
-Definition ctx := seq type.
-Local Notation "Gamma `_ i" := (get Gamma i).
-
+Definition ctx := list (term Ty)
+.
 Inductive has_type (Gamma : ctx) : term -> type -> Prop :=
 | ty_var (x : var) :
     x < size Gamma -> has_type Gamma (TeVar x) Gamma`_x
@@ -191,7 +749,3 @@ Proof.
   move=> /soundness_nil[v _ /= [t {s v} _ /(_ (fun _ => False) (TyVar 0))]].
   by move=> [s {t} _ []].
 Qed.
-
-(* Local Variables: *)
-(* coq-load-path: (("." "Ssr")) *)
-(* End: *)
