theories/Classes.v
@@ -1,0 +1,147 @@
+
+(** Type classes and notations for substitutions. *)
+Require Import Autosubst.Basics Autosubst.MMap Autosubst.Decidable Autosubst.Sorts.
+
+Notation substitution term := (vec (fun o => var -> term o)).
+
+
+(**
+  [_bind] is used to annotate the position of binders in inductive
+  definitions of syntactic objects
+ *)
+Definition _bind {sort : Set} (o : sort) (T : Type) (n : nat) := T.
+Arguments _bind / {sort} o T n.
+
+Notation "{ 'bind' n 'of' o 'in' T }" :=
+  (_bind o T n) (at level 0,
+   format "{ 'bind'  n  'of'  o  'in'  T }") : bind_scope.
+
+Notation "{ 'bind' o 'in' T }" :=
+  (_bind o T 1) (at level 0,
+                   format "{ 'bind'  o  'in'  T }") : bind_scope.
+
+Notation "{ 'bind' T }" :=
+  (_bind Sort1_1 T 1) (at level 0,
+   format "{ 'bind'  T }") : bind_scope.
+
+Open Scope bind_scope.
+
+(**
+  Classes for the substitution operations.
+
+  We use singleton classes to obtain the right reduction behaviour with simpl.
+  This relies on the feature of simpl which folds fix-bodies.
+ *)
+
+Section SubstOps.
+  Context {sort : Type}
+          {dec_eq_sort : forall a b : sort, Dec (a = b)}.
+
+  Definition upd (o : sort) {T : sort -> Type} (x : T o) (f : forall o, T o) : forall o, T o.
+    refine (fun o' => match decide (o = o') with
+                       | left p => _
+                       | right _ => f o' end).
+    subst. exact x.
+  Defined.
+  Global Arguments upd !o {T} x f !o0/.
+  Context {Vector_sort : Vector sort}.
+
+  Lemma upd_upd o {T : sort -> Type} (x y n: T o) f : upd o x (upd o y f) = upd o x f.
+  Proof.  f_ext. intro o'. unfold upd. decide(o = o'); now subst.  Qed.
+
+  Definition updV (o : sort) {term : sort -> Type} (sigma : var -> term o) (v : substitution term) : substitution term :=
+    newV (upd o sigma (getV v)).
+  Global Arguments updV o {term} sigma v.
+
+  Definition mapV {term : sort -> Type} (f : forall o, (var -> term o) -> (var -> term o)) (v : substitution term) : substitution term :=
+    newV (fun o => f o (getV v o)).
+  Global Arguments mapV {term} f v.
+
+  Definition funcompV {term : sort -> Type} (v : substitution term) (f : forall o, term o -> term o) : substitution term := @mapV term (fun o x => x >> (f o)) v.
+  Global Arguments funcompV {term} v f.
+
+  Context (term : sort -> Type).
+
+  Class Ids := ids : (forall o, var -> term o).
+  Class Rename := rename : (sort -> var -> var) -> forall o : sort, term o -> term o.
+  Class Subst := subst : (substitution term) -> forall {o : sort}, term o -> term o.
+
+End SubstOps.
+Arguments ids {sort term Ids} o x.
+Arguments rename {sort term Rename} xi [o] !s/.
+Arguments subst {sort Vector_sort term Subst} sigma [o] !s/.
+
+
+Notation "v |>> f" := (funcompV v f)
+  (at level 56, right associativity) : subst_scope.
+
+Notation "s .[ sigma ]" := (subst sigma s)
+  (at level 2, sigma at level 200, left associativity,
+   format "s .[ sigma ]" ) : subst_scope.
+
+Notation "s ..[ sigma ]" := (mmap (subst sigma) s)
+  (at level 2, sigma at level 200, left associativity,
+   format "s ..[ sigma ]" ) : subst_scope.
+
+
+
+
+Section Classes.
+
+  Context {sort : Type}
+          {dec_eq_sort : forall a b : sort, Dec (a = b)}.
+  Context {Vector_sort : Vector sort}.
+
+  Context (term : sort -> Type).
+
+  Context {Ids_term : Ids term} {Rename_term : Rename term} {Subst_term : Subst term}.
+
+
+  Definition idr : sort -> var -> var := fun _ => id.
+
+  (** Coercion from renamings to substitutions. *)
+
+  Definition renV (xi : sort -> var -> var) := newV (xi >>2 ids).
+
+
+  (** Modify a substitution when going below a binder. *)
+
+
+  Definition up (o : sort) (sigma : substitution term) : substitution term :=
+    updV o (ids o 0 .: getV sigma o >> rename (upd o (+1) idr) (o := _)) (sigma |>> rename (upd o (+1) idr)).
+  Global Arguments up o sigma : simpl never.
+
+  Notation upn := (iterate up).
+
+  Definition upren (o : sort) (xi : sort -> var -> var) : sort -> var -> var :=
+    upd o (0 .: (xi o >> S)) xi.
+  Global Arguments upren o xi o' x/.
+
+
+  (** the essential substitution lemmas *)
+
+
+ Class SubstLemmas  :=
+    {
+      rename_subst (xi : sort -> var -> var) (o : sort) (s : term o) :
+        rename xi s = subst (renV xi) s;
+      subst_id (o : sort) (s : term o) :
+        s.[newV ids] = s;
+      id_subst (sigma : substitution term) (o : sort) (x : var) :
+        (ids o x).[sigma] = getV sigma o x;
+      subst_comp (sigma tau : substitution term) (o : sort) (s : term o) :
+        s.[sigma].[tau] = s.[sigma |>> subst tau]
+    }.
+
+End Classes.
+Arguments up {sort dec_eq_sort Vector_sort term Ids_term Rename_term} o sigma : simpl never.
+Arguments renV {sort Vector_sort term Ids_term} xi : simpl never.
+Arguments SubstLemmas {sort Vector_sort} term {Ids_term Rename_term Subst_term}.
+
+Arguments idr {sort} o/ x.
+
+Arguments newV : simpl never.
+Arguments getV {sort Vector T} v o.
+Arguments funcompV {sort Vector_sort term} !v f.
+
+Notation ren xi := (xi >> ids _).
