theories/Derive.v
@@ -1,0 +1,223 @@
+(** Tactics to generate substitution operations and show the basic lemmas. *)
+From Autosubst Require Import Basics MMap Classes Tactics Decidable.
+
+(* Ltac app_var := match goal with [ |- var] => assumption end. *)
+
+(* Ltac derive_Ids := intro;  solve *)
+(*   [ constructor 1; [app_var] | constructor 2; [app_var] *)
+(*   | constructor 3; [app_var] | constructor 4; [app_var] *)
+(*   | constructor 5; [app_var] | constructor 6; [app_var] *)
+(*   | constructor 7; [app_var] | constructor 8; [app_var] *)
+(*   | constructor 9; [app_var] | constructor 10; [app_var] *)
+(*   | constructor 11; [app_var] | constructor 12; [app_var] *)
+(*   | constructor 13; [app_var] | constructor 14; [app_var] *)
+(*   | constructor 15; [app_var] | constructor 16; [app_var] *)
+(*   | constructor 17; [app_var] | constructor 18; [app_var] *)
+(*   | constructor 19; [app_var] | constructor 20; [app_var]]. *)
+(* Hint Extern 0 (Ids _) => derive_Ids : derive. *)
+
+
+Ltac derive_Rename :=
+  match goal with [ |- Rename ?term ] =>
+    hnf; fix inst 3; change _ with (Rename term) in inst;
+    intros xi o s; change (annot (term o) s); destruct s;
+    match goal with
+      | [ x : var |- annot _ (?Var _ _)] => exact (Var o (xi o x))
+      | [ |- annot _ ?t ] =>
+        let rec map s :=
+            (match s with
+               | ?s1 ?s2 =>
+                 let s1 := map s1 in
+                 let T  := typeof s2 in
+                 let s2 :=
+                     match T with
+                       | term _ => constr:(rename xi s2)
+                       | var  => constr:(xi s2)
+                       | @_bind _ ?o _ 1 => constr:(rename (upren o xi) s2)
+                       | @_bind _ ?o _ ?n =>
+                           constr:(rename (iterate (upren o) n xi) s2)
+                       | _ => s2
+                     end in
+                 constr:(s1 s2)
+               | _ => s
+             end) in
+        let t := map t in exact t
+    end
+  end.
+Hint Extern 0 (Rename _) => derive_Rename : derive.
+
+
+Ltac has_var s :=
+  match s with
+    | ?s1 ?s2 =>
+      match has_var s1 with
+        | Some ?x => constr:(Some x)
+        | _ =>
+          match typeof s2 with
+            | var => constr:(Some s2)
+            | _ => None
+          end
+      end
+    | _ => None
+  end.
+
+Ltac derive_Subst :=
+  match goal with [ |- Subst ?term ] =>
+    require_instance (Rename term);
+    hnf; fix inst 3; change _ with (Subst term) in inst;
+    intros sigma o s; change (annot (term o) s); destruct s;
+    match goal with
+      | [ x : var |- annot _ (?Var _ _)] =>
+        exact (getV sigma o x)
+      | [ |- annot _ ?t ] =>
+        let rec map s :=
+            (match s with
+               | ?s1 ?s2 =>
+                 let s1 := map s1 in
+                 let T  := typeof s2 in
+                 let s2 :=
+                   match T with
+                     | term _ => constr:(s2.[sigma])
+                     | _bind ?o _ 1 => constr:(s2.[up o sigma])
+                     | _bind ?o _ ?n => constr:(s2.[iterate (up o) n sigma])
+                   end in
+                 constr:(s1 s2)
+               | _ => s
+             end) in
+        let t := map t in exact t
+    end
+  end.
+Hint Extern 0 (Subst _) => derive_Subst : derive.
+
+
+Lemma mmap_id_ext {A B} {inst : MMap A B} `{@MMapLemmas A B inst}
+  `{@MMapExt A B inst} (f : A -> A) (b : B) :
+  (forall x, f x = x) -> mmap f b = b.
+Proof. intros E. rewrite (mmap_ext E). apply mmap_id. Defined.
+
+Lemma iter_fp {A} (f : A -> A) x :
+  f x = x -> forall n, iterate f n x = x.
+Proof.
+  intros E. induction n. reflexivity. rewrite iterate_S. simpl. now rewrite IHn.
+Qed.
+
+Lemma iter_param {A B} (f : A -> A) (g : B -> B) (h : A -> B) :
+  (forall x, g (h x) = h (f x)) ->
+  (forall x n, iterate g n (h x) = h (iterate f n x)).
+Proof.
+  intros E x n. induction n. reflexivity. rewrite !iterate_S. simpl. now rewrite IHn, E.
+Qed.
+
+Ltac casedist_up := intros o; intros; simpl; destruct o; unfold up; unfold renV; unfold newV; unfold funcompV; simpl; f_equal; f_ext; (intros [|x]); reflexivity.
+
+Section SubstLemmasInternal.
+
+  Context {sort : Set} {decide_eq_sort : forall a b : sort, Dec (a = b)} {Vector_sort : Vector sort}.
+  Context {term : sort -> Type}
+          {Ids_term : Ids term} {Rename_term : Rename term} {Subst_term : Subst term}
+          {SubstLemmas_term : SubstLemmas term}.
+
+Lemma up_comp_subst_ren_n_internal :
+  (forall o sigma xi, up o (sigma |>> rename xi) = up o sigma |>> rename (upren o xi))->
+  (forall o sigma xi n,
+    iterate (up o) n (sigma |>> rename xi) = iterate (up o) n sigma |>> rename (iterate (upren o) n xi)).
+Proof.
+  intros E o sigma xi n. induction n. reflexivity. rewrite !iterate_S. simpl. now rewrite IHn.
+Qed.
+
+Lemma up_comp_ren_subst o xi sigma :
+    up o (newV (xi >>2 getV sigma)) = newV (upren o xi >>2 getV (up o sigma)).
+Proof.
+  unfold up. unfold updV. f_equal. f_ext. intros o'. f_ext. simpl.
+  unfold funcompV. unfold mapV. rewrite ?getV_newV.
+  unfold upd.
+  decide (o=o'); simpl.
+  - unfold eq_rect_r. unfold eq_rect. destruct eq_sym. now intros [|x].
+  - now intros [|x].
+Qed.
+
+Lemma up_comp_ren_subst_n o xi sigma n :
+  iterate (up o) n (newV (xi >>2 getV sigma)) = newV (iterate (upren  o) n xi >>2 getV (iterate (up o) n sigma)) .
+Proof.
+  induction n. reflexivity. rewrite !iterate_S. simpl. rewrite IHn. apply up_comp_ren_subst.
+Qed.
+
+End SubstLemmasInternal.
+
+Ltac derive_SubstLemmas :=
+  lazymatch goal with
+    [ |-
+@SubstLemmas ?sort ?Vector_sort ?term ?Ids_term ?Rename_term ?Subst_term] =>
+
+    (* rename subst *)
+
+assert (rename_subst :
+          forall o xi (s : term o), rename xi s = subst (renV xi) s)
+  by (
+      assert (up_upren :
+                forall o xi, up o (renV xi) = renV (upren o xi))
+      by casedist_up;
+      assert (up_upren_n :
+                forall o xi n, iterate (up o) n (renV xi) = renV (iterate (upren o) n xi))
+        by (intros; now apply iter_param);
+      fix ih 3; intros o xi s; destruct s; (try destruct o); try reflexivity; try (simpl; f_equal ;
+                                                                                  try apply mmap_ext; intros; rewrite ?up_upren, ?up_upren_n; now apply ih));
+
+  (* subst id *)
+
+  assert (subst_id : forall o (s : term o), subst (newV ids) s = id s)
+  by (
+      assert (up_id : forall o, up o (newV ids) = newV ids) by casedist_up;
+      assert (up_id_n : forall o n, iterate (up o) n (newV ids) = (newV ids)) by (intros; now apply iter_fp);
+      fix ih 2; intros o s; destruct s; simpl in *; repeat match goal with [o : sort |- _ ] => destruct o end; f_equal; try reflexivity;
+      rewrite ?up_id, ?up_id_n; try apply mmap_id_ext; intros; apply ih);
+
+  (* subst comp *)
+
+  assert (ren_subst_comp :
+            forall (xi : sort -> var -> var) sigma o (s : term o), (rename xi s).[sigma] = s.[newV (xi >>2 getV sigma)])
+    by (
+        fix ih 4; intros xi sigma o s; destruct s; simpl; trivial; try
+        (now destruct o); now (
+        f_equal; rewrite ?up_comp_ren_subst, ?up_comp_ren_subst_n, ?mmap_comp;
+               try apply mmap_ext; intros; try apply ih)
+      );
+
+  assert (subst_ren_comp : forall sigma xi o (s : term o),
+                             rename xi s.[sigma] = s.[sigma |>> rename xi])
+    by (
+
+        assert (up_comp_subst_ren :
+                  forall o sigma xi, up o (sigma |>> rename xi) = up o sigma |>> rename (upren o xi))
+        by (
+            intros o sigma xi; destruct sigma; destruct o; simpl; unfold up; unfold funcompV; simpl; repeat first[f_ext | f_equal]; destruct 0; trivial; simpl; try now repeat rewrite rename_subst, ren_subst_comp);
+
+        assert (up_comp_subst_ren_n :
+                  forall o sigma xi n, iterate (up o) n (sigma |>> rename xi) = iterate (up o) n sigma |>> rename (iterate (upren o) n xi))
+          by (
+              apply up_comp_subst_ren_n_internal; apply up_comp_subst_ren);
+        fix ih 4; intros sigma xi o s; destruct s; try reflexivity; simpl;
+        f_equal; rewrite ?up_comp_subst_ren, ?up_comp_subst_ren_n, ?mmap_comp;
+        first [now destruct o | intros; apply ih]
+      );
+
+assert (subst_comp :
+          forall o sigma tau (s : term o), s.[sigma].[tau] = s.[sigma |>> subst tau])
+  by (
+      assert (up_comp : forall o sigma tau, up o (sigma |>> subst tau) = up o sigma |>> subst (up o tau))
+      by (
+          intros o sigma tau; destruct o; unfold up; unfold funcompV; simpl;
+          repeat first[f_ext | f_equal] ;
+          destruct 0; simpl; trivial; rewrite ?subst_ren_comp; now rewrite ?ren_subst_comp
+        );
+
+      (* assert (up_comp_n : forall sigma tau n, upn n (sigma >> tau) = upn n sigma >> upn n tau) *)
+      (*  by (apply up_comp_n_internal; apply up_comp); *)
+      fix ih 4; intros o sigma tau s; destruct s; simpl; trivial; simpl; f_equal;
+      rewrite ?up_comp, (*?up_comp_n, *) ?mmap_comp;
+      try apply mmap_ext; intros; solve[ now destruct o | apply ih]
+    );
+constructor; hnf; intros;
+[apply rename_subst|apply subst_id|reflexivity|apply subst_comp]
+  end.
+Hint Extern 0 (SubstLemmas _) => derive_SubstLemmas : derive.
