theories/Tactics.v
@@ -1,0 +1,197 @@
+(** The main automation tactics. *)
+Require Import Autosubst.Basics Autosubst.Decidable Autosubst.MMap Autosubst.Classes.
+
+(** Derived substitution lemmas. *)
+
+Section LemmasForSubst.
+
+  Context {sort : Type}
+          {dec_eq_sort : forall a b : sort, Dec (a = b)}
+          {Vector_sort : Vector sort}
+          {term : sort -> Type}
+          {Ids_term : Ids term} {Rename_term : Rename term} {Subst_term : Subst term}
+          {SubstLemmas_term : SubstLemmas term}.
+
+Implicit Types (sigma tau theta :  substitution term) (xi : sort -> var -> var).
+
+Lemma rename_substX xi : rename xi = subst (renV xi).
+Proof. repeat(f_ext; intros). now apply rename_subst. Qed.
+
+(* Variable (o : sort) (sigma : vec (fun o : sort => var -> term o)) (s : term o) . *)
+
+(* Goal up o sigma = up o sigma. unfold up. simpl. rewrite rename_substX. simpl. *)
+
+Lemma upX o (sigma : substitution term) :
+  up o sigma =
+  updV o (ids o 0 .: getV sigma o >> subst (renV (upd o (+1) idr)) (o:=o))
+     (sigma |>> subst (renV (upd o (+1) idr))).
+Proof. unfold up. now rewrite rename_substX. Qed.
+
+Lemma id_scompX sigma o : ids o >> subst sigma (o := o) = getV sigma o.
+Proof. f_ext. now eapply id_subst. Qed.
+
+Lemma id_scompR {A} sigma o (f : term o -> A) :
+  ids o >> (subst sigma (o := o) >> f) = getV sigma o >> f.
+Proof. now rewrite <- compA, id_scompX. Qed.
+
+Lemma subst_idX : subst (newV ids) = fun o (s : term o) => s.
+Proof. f_ext. intro. f_ext. now eapply subst_id. Qed.
+
+Lemma subst_compI sigma tau o (s : term o) :
+  s.[sigma].[tau] = s.[sigma |>> subst tau].
+Proof. now eapply subst_comp. Qed.
+
+Lemma subst_compX sigma tau o :
+  subst sigma (o := o) >> subst tau (o := o) = subst (sigma |>> subst tau) (o := o).
+Proof. f_ext. intro. now eapply subst_comp. Qed.
+
+(* Lemma subst_compR {A} sigma tau (f : _ -> A) : *)
+(*   subst sigma >> (subst tau >> f) = subst (sigma >> subst tau) >> f. *)
+(* Proof. now rewrite <- subst_compX. Qed. *)
+
+Lemma fold_ren_cons (x : var) (xi : var -> var) o :
+  ids o x .: (xi >> ids o) = (x .: xi) >> ids o.
+Proof. now rewrite scons_comp. Qed.
+
+(* unfold upn *)
+
+(* Lemma upnSX n sigma : *)
+(*   upn (S n) sigma = ids 0 .: upn n sigma >> subst (ren (+1)). *)
+(* Proof. *)
+(*   unfold iterate; now rewrite upX. *)
+(* Qed. *)
+
+(* Lemma upnSE n sigma : *)
+(*   upn (S n) sigma = ids 0 .: upn n sigma >> ren (+1). *)
+(* Proof. *)
+(*   now rewrite upnSX. *)
+(* Qed. *)
+
+(* Lemma upn0 sigma : upn 0 sigma = sigma. *)
+(* Proof. reflexivity. Qed. *)
+
+
+
+(* fold up *)
+
+(* Lemma fold_up k sigma : *)
+(*   ids k .: sigma >> ren (+S k) = up sigma >> ren (+k). *)
+(* Proof. *)
+(*   unfold scomp, ren. rewrite upX; fsimpl; rewrite id_subst, subst_compX; simpl; fsimpl. *)
+(*   unfold ren. fsimpl. rewrite id_scompX. now fsimpl. *)
+(* Qed. *)
+
+(* Lemma fold_up0 sigma : *)
+(*   sigma >> ren (+0) = sigma. *)
+(* Proof. *)
+(*   unfold scomp, ren. fsimpl. now rewrite subst_idX. *)
+(* Qed. *)
+
+
+
+(* combine up *)
+
+(* Lemma fold_up_up sigma : up (up sigma) = upn 2 sigma. *)
+(* Proof. reflexivity. Qed. *)
+
+(* Lemma fold_up_upn n sigma : up (upn n sigma) = upn (S n) sigma. *)
+(* Proof. reflexivity. Qed. *)
+
+(* Lemma fold_upn_up n sigma : upn n (up sigma) = upn (S n) sigma. *)
+(* Proof. now rewrite iterate_Sr. Qed. *)
+
+End LemmasForSubst.
+
+Ltac autosubst_fold := rewrite <- ?compA, -> ?fold_ren_cons.
+
+Ltac autosubst_typeclass_normalize :=
+  mmap_typeclass_normalize;
+  repeat match goal with
+  | [|- context[ids ?x]] =>
+    let s := constr:(ids x) in progress change (ids x) with s
+  | [|- appcontext[renV ?xi]] =>
+    let s := constr:(renV xi) in progress change (renV xi) with s
+  | [|- appcontext[rename ?xi]] =>
+    let s := constr:(rename xi) in progress change (rename xi) with s
+  | [|- appcontext[subst ?sigma]] =>
+    let s := constr:(subst sigma) in progress change (subst sigma) with s
+  end.
+
+Ltac autosubst_typeclass_normalizeH H :=
+  mmap_typeclass_normalizeH H;
+  repeat match typeof H with
+  | context[ids ?x] =>
+    let s := constr:(ids x) in progress change (ids x) with s in H
+  | appcontext[renV ?xi] =>
+    let s := constr:(renV xi) in progress change (renV xi) with s in H
+  | appcontext[rename ?xi] =>
+    let s := constr:(rename xi) in progress change (rename xi) with s in H
+  | appcontext[subst ?sigma] =>
+    let s := constr:(subst sigma) in progress change (subst sigma) with s in H
+  end.
+
+
+Ltac autosubst_unfold_up :=
+  rewrite ?upX (*, ?upnSX; *)
+  (* repeat match goal with *)
+  (* | [|- context[upn 0 ?sigma]] => change (upn 0 sigma) with sigma *)
+  (* end *).
+
+Ltac autosubst_unfold_upH H :=
+  rewrite ?upX(* , ?upnSX*) in H(*; *)
+  (* repeat match typeof H with *)
+  (* | context[upn 0 ?sigma] => change (upn 0 sigma) with sigma *)
+  (* end *).
+
+Ltac autosubst_unfold :=
+  autosubst_typeclass_normalize; autosubst_unfold_up;
+  rewrite ?(@rename_substX _ _ _ _ _ _); unfold renV, upren, newV.
+
+Ltac autosubst_unfoldH H :=
+  autosubst_typeclass_normalizeH H; autosubst_unfold_upH H;
+  rewrite ?(@rename_substX _ _ _ _ _ _) in H; unfold renV, upren, newV in H.
+
+Ltac etaReduce := repeat lazymatch goal with [|- context[fun x => ?f x]] => change (fun x => f x) with f end.
+
+Ltac etaReduceH H := repeat lazymatch goal with [H : context[fun x => ?f x] |- _ ] => change (fun x => f x) with f in H end.
+
+Ltac asimpl := fsimpl; try
+  let subst_idX_inst := fresh "E" in
+  lazymatch goal with [|- appcontext[@subst _ _ _ ?Subst_term]] =>
+pose proof (@subst_idX _ _ _ _ _ Subst_term _) as subst_idX_inst;
+  unfold newV in subst_idX_inst;
+  simpl in subst_idX_inst
+  end;
+  simpl; autosubst_unfold; repeat first
+  [ progress (
+      simpl; unfold _bind, renV, funcompV; fsimpl; autosubst_unfold_up;
+      autorewrite with autosubst;
+      rewrite ?id_scompX, ?id_scompR, ?subst_compX,
+      (* ?subst_compR, *) ?id_subst, ?subst_id, ?subst_compI, ?subst_idX_inst
+      (* repeat match goal with [|- appcontext[@subst ?sort ?vec ?term ?Subst ?sigma]] => *)
+      (*                        replace (@subst sort vec term Subst sigma ) with (fun o : sort =>  @id (term o)) by eauto using subst_idX end *)
+    )
+  | fold_id];
+  autosubst_fold;
+  clear subst_idX_inst
+.
+
+Ltac autosubst := now asimpl.
+
+Ltac asimplH H :=
+  simpl in H; autosubst_unfoldH H; repeat first
+  [ progress (
+        simpl in H;
+        unfold _bind, renV, funcompV in H; fsimplH H;
+        autosubst_unfold_upH H;
+        autorewrite with autosubst in H;
+        rewrite ?id_scompX, ?id_scompR, ?subst_compX,
+        (* ?subst_compR, *) ?id_subst, ?subst_id in H;
+        repeat setoid_rewrite subst_compI in H;
+        let E := constr:(@subst_idX _ _ _ _ _ _) in rewrite ?(E _ _) in H (* I have no idea why this works ... well, it does no longer in Coq 8.5*)
+      )
+  | fold_idH H](* ; *)
+(* fold_ren; fold_comp; fold_up *).
+
+Tactic Notation "asimpl" "in" ident(H) := asimplH H.
+Tactic Notation "asimpl" "in" "*" := (in_all asimplH); asimpl.
